lib/generic_bv_ops.dfy
@@ -72,6 +72,9 @@ abstract module generic_bv_ops
 
     function method xor(x: uint, y: uint): uint
 
+    lemma xor_clear_lemma(x: uint)
+        ensures xor(x, x) == 0;
+
     predicate valid_shift(amount: uint)
 
     function method rs(x: uint, amount: uint): uint
